theories/STac/Core.v
@@ -1,5 +1,7 @@
 Require Import Coq.Lists.List.
 Require Import ExtLib.Core.RelDec.
+Require Import ExtLib.Structures.Traversable.
+Require Import ExtLib.Data.List.
 Require Import ExtLib.Tactics.
 Require Import MirrorCore.EnvI.
 Require Import MirrorCore.SymI.
@@ -18,12 +20,12 @@ Section parameterized.
 
   Inductive Result : Type :=
   | Fail
+      (** TODO: Should [Solved] not have extended environments? **)
   | Solved : list typ -> list typ -> subst -> Result
-  | More : list typ -> list typ -> subst -> expr -> Result.
+  | More : list typ -> list typ -> subst -> list expr -> expr -> Result.
 
   Definition stac : Type :=
-    (** TODO: Part of the state is hypotheses **)
-    list typ -> list typ -> subst -> expr ->
+    list typ -> list typ -> subst -> list expr -> expr ->
     Result.
 
   Variable RType_typ : RType typ.
@@ -42,70 +44,79 @@ Section parameterized.
     end.
 
   Definition stac_sound (tac : stac) : Prop
-  := forall tus tvs s (g : expr),
+  := forall tus tvs s (hs : list expr) (g : expr),
        WellFormed_subst s ->
-       match tac tus tvs s g with
+       match tac tus tvs s hs g with
          | Fail => True
          | Solved tus' tvs' s' =>
            WellFormed_subst s' /\
            match goalD tus tvs g
+               , mapT (F:=option) (T:=list) (goalD tus tvs) hs
                , substD tus tvs s
            with
-             | Some G , Some sV =>
+             | Some G , Some Hs , Some sV =>
                match substD (tus ++ tus') (tvs ++ tvs') s' with
                  | None => False
                  | Some s'V =>
-                   forall us vs,
+                   forall (us : HList.hlist _ tus) (vs : HList.hlist _ tvs),
                      (exists us' vs',
                         s'V (HList.hlist_app us us') (HList.hlist_app vs vs')) ->
+                     Forall (fun P => P us vs) Hs ->
                      G us vs /\ sV us vs
                end
-             | _ , _ => True
+             | _ , _ , _ => True
            end
-         | More tus' tvs' s' g' =>
+         | More tus' tvs' s' hs' g' =>
            WellFormed_subst s' /\
            match goalD tus tvs g
+               , mapT (F:=option) (T:=list) (goalD tus tvs) hs
                , substD tus tvs s
            with
-             | Some G , Some sV =>
+             | Some G , Some Hs , Some sV =>
                match goalD (tus ++ tus') (tvs ++ tvs') g'
+                   , mapT (F:=option) (T:=list) (goalD (tus ++ tus') (tvs ++ tvs')) hs'
                    , substD (tus ++ tus') (tvs ++ tvs') s'
                with
-                 | Some G' , Some s'V =>
+                 | Some G' , Some Hs' , Some s'V =>
                    forall us vs,
                      (exists us' vs',
-                           s'V (HList.hlist_app us us') (HList.hlist_app vs vs')
-                        /\ G' (HList.hlist_app us us') (HList.hlist_app vs vs')) ->
+                        let us := HList.hlist_app us us' in
+                        let vs := HList.hlist_app vs vs' in
+                        Forall (fun P => P us vs) Hs' ->
+                           s'V us vs
+                        /\ G' us vs) ->
+                     Forall (fun P => P us vs) Hs ->
                      G us vs /\ sV us vs
-                 | _ , _ => False
+                 | _ , _ , _ => False
                end
-             | _ , _ => True
+             | _ , _ , _ => True
            end
        end.
 
   Lemma More_sound
-  : forall tus tvs s g,
-      match goalD tus tvs g with
-        | Some G =>
-          match substD tus tvs s with
-            | Some sV =>
-              match goalD (tus ++ nil) (tvs ++ nil) g with
-                | Some G' =>
-                  match substD (tus ++ nil)%list (tvs ++ nil)%list s with
-                    | Some s'V =>
-                      forall (us : HList.hlist (typD nil) tus)
-                             (vs : HList.hlist (typD nil) tvs),
-                        (exists us' vs' : HList.hlist (typD nil) nil,
-                           s'V (HList.hlist_app us us') (HList.hlist_app vs vs') /\
-                           G' (HList.hlist_app us us') (HList.hlist_app vs vs')) ->
-                        G us vs /\ sV us vs
-                    | None => False
-                  end
-                | None => False
-              end
-            | None => True
+  : forall tus tvs s hs g,
+      match goalD tus tvs g
+          , mapT (F:=option) (T:=list) (goalD tus tvs) hs
+          , substD tus tvs s
+      with
+        | Some G , Some Hs , Some sV =>
+          match goalD (tus ++ nil) (tvs ++ nil) g
+              , mapT (F:=option) (T:=list) (goalD (tus ++ nil) (tvs ++ nil)) hs
+              , substD (tus ++ nil)%list (tvs ++ nil)%list s
+          with
+            | Some G' , Some Hs' , Some s'V =>
+              forall (us : HList.hlist (typD nil) tus)
+                     (vs : HList.hlist (typD nil) tvs),
+                (exists us' vs' : HList.hlist (typD nil) nil,
+                   let us := HList.hlist_app us us' in
+                   let vs := HList.hlist_app vs vs' in
+                   Forall (fun P => P us vs) Hs' ->
+                   s'V us vs /\ G' us vs) ->
+                Forall (fun P => P us vs) Hs ->
+                G us vs /\ sV us vs
+            | _ , _ , _ => False
           end
-        | None => True
+        | _ , _ , _ => True
       end.
   Proof.
     intros.
@@ -114,18 +125,21 @@ Section parameterized.
              | |- match ?X with _ => _ end =>
                consider X; intros
            end.
-    { destruct H3 as [ ? [ ? ? ] ].
+    { destruct H5 as [ ? [ ? ? ] ].
       rewrite (HList.hlist_eta x) in *.
       rewrite (HList.hlist_eta x0) in *.
-      do 2 rewrite HList.hlist_app_nil_r in H3.
+      do 2 rewrite HList.hlist_app_nil_r in H5.
       destruct (eq_sym (HList.app_nil_r_trans tus)).
       destruct (eq_sym (HList.app_nil_r_trans tvs)).
-      rewrite H0 in *.
-      rewrite H1 in *. inv_all; subst.
+      rewrite H0 in *. rewrite H1 in *. rewrite H in *.
+      inv_all; subst.
+      simpl in H5. eapply H5 in H6.
       tauto. }
-    { do 2 rewrite List.app_nil_r in H2.
+    { do 2 rewrite List.app_nil_r in *.
       congruence. }
-    { do 2 rewrite List.app_nil_r in H1.
+    { do 2 rewrite List.app_nil_r in *.
+      congruence. }
+    { do 2 rewrite List.app_nil_r in *.
       congruence. }
   Qed.
 
