theories/STac/Try.v
@@ -9,9 +9,9 @@ Section parameterized.
   Variable subst : Type.
 
   Definition TRY (b : stac typ expr subst) : stac typ expr subst :=
-    fun tus tvs sub e =>
-      match b tus tvs sub e with
-        | Fail => More nil nil sub e
+    fun tus tvs sub hs e =>
+      match b tus tvs sub hs e with
+        | Fail => More nil nil sub hs e
         | x => x
       end.
 
@@ -25,8 +25,8 @@ Section parameterized.
   Theorem TRY_sound : forall b, stac_sound b -> stac_sound (TRY b).
   Proof.
     unfold stac_sound; intros.
-    specialize (H tus tvs s g). unfold TRY.
-    destruct (b tus tvs s g); auto.
+    specialize (H tus tvs s hs g). unfold TRY.
+    destruct (b tus tvs s hs g); auto.
     split; auto.
     apply More_sound.
   Qed.
