theories/STac/Solve.v
@@ -9,8 +9,8 @@ Section parameterized.
   Variable subst : Type.
 
   Definition SOLVE (b : stac typ expr subst) : stac typ expr subst :=
-    fun e sub tus tvs =>
-      match b e sub tus tvs with
+    fun tus tvs sub hs e =>
+      match b tus tvs sub hs e with
         | Solved tus tvs s => @Solved _ _ _ tus tvs s
         | x => @Fail _ _ _
       end.
@@ -25,8 +25,8 @@ Section parameterized.
   Theorem SOLVE_sound : forall t, stac_sound t -> stac_sound (SOLVE t).
   Proof.
     unfold stac_sound; simpl; intros.
-    red. specialize (H tus tvs s g).
-    destruct (t tus tvs s g); auto.
+    red. specialize (H tus tvs s hs g).
+    destruct (t tus tvs s hs g); auto.
   Qed.
 
 End parameterized.
